Fine-grained post-conditions for forked-off threads.
This commit extends the state interpretation with an additional parameter to
talk about the number of forked-off threads, and a fixed postcondition for each
forked-off thread:

    state_interp : Λstate → list Λobservation → nat → iProp Σ;
    fork_post : iProp Σ;

This way, instead of having `True` as the post-condition of `Fork`, one can
have any post-condition, which is then recorded in the state interpretation.
The point of keeping track of the postconditions of forked-off threads, is that
we get an (additional) stronger adequacy theorem:

    Theorem wp_strong_all_adequacy Σ Λ `{invPreG Σ} s e σ1 v vs σ2 φ :
       (∀ `{Hinv : invG Σ} κs,
         (|={⊤}=> ∃
             (stateI : state Λ → list (observation Λ) → nat → iProp Σ)
             (fork_post : iProp Σ),
           let _ : irisG Λ Σ := IrisG _ _ _ Hinv stateI fork_post in
           stateI σ1 κs 0 ∗ WP e @ s; ⊤ {{ v,
             let m := length vs in
             stateI σ2 [] m -∗ [∗] replicate m fork_post ={⊤,∅}=∗ ⌜ φ v ⌝ }})%I) →
      rtc erased_step ([e], σ1) (of_val <$> v :: vs, σ2) →
      φ v.

The difference with the ordinary adequacy theorem is that this one only applies
once all threads terminated. In this case, one gets back the post-conditions
`[∗] replicate m fork_post` of all forked-off threads.

In Iron we showed that we can use this mechanism to make sure that all
resources are disposed of properly in the presence of fork-based concurrency.

theories/program_logic/total_adequacy.v
@@ -11,16 +11,17 @@ Implicit Types e : expr Λ.
 
 Definition twptp_pre (twptp : list (expr Λ) → iProp Σ)
     (t1 : list (expr Λ)) : iProp Σ :=
-  (∀ t2 σ1 κ κs σ2, ⌜step (t1,σ1) κ (t2,σ2)⌝ -∗
-    state_interp σ1 κs ={⊤}=∗ ⌜κ = []⌝ ∗ state_interp σ2 κs ∗ twptp t2)%I.
+  (∀ t2 σ1 κ κs σ2 n, ⌜step (t1,σ1) κ (t2,σ2)⌝ -∗
+    state_interp σ1 κs n ={⊤}=∗ ∃ n', ⌜κ = []⌝ ∗ state_interp σ2 κs n' ∗ twptp t2)%I.
 
 Lemma twptp_pre_mono (twptp1 twptp2 : list (expr Λ) → iProp Σ) :
   (<pers> (∀ t, twptp1 t -∗ twptp2 t) →
   ∀ t, twptp_pre twptp1 t -∗ twptp_pre twptp2 t)%I.
 Proof.
   iIntros "#H"; iIntros (t) "Hwp". rewrite /twptp_pre.
-  iIntros (t2 σ1 κ κs σ2) "Hstep Hσ". iMod ("Hwp" with "[$] [$]") as "[$ [$ ?]]".
-  by iApply "H".
+  iIntros (t2 σ1 κ κs σ2 n1) "Hstep Hσ".
+  iMod ("Hwp" with "[$] [$]") as (n2) "($ & Hσ & ?)".
+  iModIntro. iExists n2. iFrame "Hσ". by iApply "H".
 Qed.
 
 Local Instance twptp_pre_mono' : BiMonoPred twptp_pre.
@@ -49,9 +50,10 @@ Instance twptp_Permutation : Proper ((≡ₚ) ==> (⊢)) twptp.
 Proof.
   iIntros (t1 t1' Ht) "Ht1". iRevert (t1' Ht); iRevert (t1) "Ht1".
   iApply twptp_ind; iIntros "!#" (t1) "IH"; iIntros (t1' Ht).
-  rewrite twptp_unfold /twptp_pre. iIntros (t2 σ1 κ κs σ2 Hstep) "Hσ".
+  rewrite twptp_unfold /twptp_pre. iIntros (t2 σ1 κ κs σ2 n Hstep) "Hσ".
   destruct (step_Permutation t1' t1 t2 κ σ1 σ2) as (t2'&?&?); try done.
-  iMod ("IH" $! t2' with "[% //] Hσ") as "($ & $ & IH & _)". by iApply "IH".
+  iMod ("IH" $! t2' with "[% //] Hσ") as (n2) "($ & Hσ & IH & _)".
+  iModIntro. iExists n2. iFrame "Hσ". by iApply "IH".
 Qed.
 
 Lemma twptp_app t1 t2 : twptp t1 -∗ twptp t2 -∗ twptp (t1 ++ t2).
@@ -60,22 +62,23 @@ Proof.
   iApply twptp_ind; iIntros "!#" (t1) "IH1". iIntros (t2) "H2".
   iRevert (t1) "IH1"; iRevert (t2) "H2".
   iApply twptp_ind; iIntros "!#" (t2) "IH2". iIntros (t1) "IH1".
-  rewrite twptp_unfold /twptp_pre. iIntros (t1'' σ1 κ κs σ2 Hstep) "Hσ1".
+  rewrite twptp_unfold /twptp_pre. iIntros (t1'' σ1 κ κs σ2 n Hstep) "Hσ1".
   destruct Hstep as [e1 σ1' e2 σ2' efs' t1' t2' ?? Hstep]; simplify_eq/=.
   apply app_eq_inv in H as [(t&?&?)|(t&?&?)]; subst.
   - destruct t as [|e1' ?]; simplify_eq/=.
-    + iMod ("IH2" with "[%] Hσ1") as "($ & $ & IH2 & _)".
+    + iMod ("IH2" with "[%] Hσ1") as (n2) "($ & Hσ & IH2 & _)".
       { by eapply step_atomic with (t1:=[]). }
-      iModIntro. rewrite -{2}(left_id_L [] (++) (e2 :: _)). iApply "IH2".
+      iModIntro. iExists n2. iFrame "Hσ".
+      rewrite -{2}(left_id_L [] (++) (e2 :: _)). iApply "IH2".
       by setoid_rewrite (right_id_L [] (++)).
-    + iMod ("IH1" with "[%] Hσ1") as "($ & $ & IH1 & _)"; first by econstructor.
+    + iMod ("IH1" with "[%] Hσ1") as (n2) "($ & Hσ & IH1 & _)"; first by econstructor.
       iAssert (twptp t2) with "[IH2]" as "Ht2".
       { rewrite twptp_unfold. iApply (twptp_pre_mono with "[] IH2").
         iIntros "!# * [_ ?] //". }
-      iModIntro. rewrite -assoc_L (comm _ t2) !cons_middle !assoc_L.
-      by iApply "IH1".
-  - iMod ("IH2" with "[%] Hσ1") as "($ & $ & IH2 & _)"; first by econstructor.
-    iModIntro. rewrite -assoc. by iApply "IH2".
+      iModIntro. iExists n2. iFrame "Hσ".
+      rewrite -assoc_L (comm _ t2) !cons_middle !assoc_L. by iApply "IH1".
+  - iMod ("IH2" with "[%] Hσ1") as (n2) "($ & Hσ & IH2 & _)"; first by econstructor.
+    iModIntro. iExists n2. iFrame "Hσ". rewrite -assoc_L. by iApply "IH2".
 Qed.
 
 Lemma twp_twptp s Φ e : WP e @ s; ⊤ [{ Φ }] -∗ twptp [e].
@@ -83,42 +86,46 @@ Proof.
   iIntros "He". remember (⊤ : coPset) as E eqn:HE.
   iRevert (HE). iRevert (e E Φ) "He". iApply twp_ind.
   iIntros "!#" (e E Φ); iIntros "IH" (->).
-  rewrite twptp_unfold /twptp_pre /twp_pre. iIntros (t1' σ1' κ κs σ2' Hstep) "Hσ1".
+  rewrite twptp_unfold /twptp_pre /twp_pre. iIntros (t1' σ1' κ κs σ2' n Hstep) "Hσ1".
   destruct Hstep as [e1 σ1 e2 σ2 efs [|? t1] t2 ?? Hstep];
     simplify_eq/=; try discriminate_list.
   destruct (to_val e1) as [v|] eqn:He1.
   { apply val_stuck in Hstep; naive_solver. }
   iMod ("IH" with "Hσ1") as "[_ IH]".
-  iMod ("IH" with "[% //]") as "($ & $ & [IH _] & IHfork)"; iModIntro.
+  iMod ("IH" with "[% //]") as "($ & Hσ & [IH _] & IHfork)".
+  iModIntro. iExists (length efs + n). iFrame "Hσ".
   iApply (twptp_app [_] with "[IH]"); first by iApply "IH".
   clear. iInduction efs as [|e efs] "IH"; simpl.
-  { rewrite twptp_unfold /twptp_pre. iIntros (t2 σ1 κ κs σ2 Hstep).
+  { rewrite twptp_unfold /twptp_pre. iIntros (t2 σ1 κ κs σ2 n1 Hstep).
     destruct Hstep; simplify_eq/=; discriminate_list. }
   iDestruct "IHfork" as "[[IH' _] IHfork]".
-  iApply (twptp_app [_] with "[IH']"); [by iApply "IH'"|by iApply "IH"].
+  iApply (twptp_app [_] with "[IH']"). by iApply "IH'". by iApply "IH".
 Qed.
 
-Lemma twptp_total σ t :
-  state_interp σ [] -∗ twptp t ={⊤}=∗ ▷ ⌜sn erased_step (t, σ)⌝.
+Lemma twptp_total n σ t :
+  state_interp σ [] n -∗ twptp t ={⊤}=∗ ▷ ⌜sn erased_step (t, σ)⌝.
 Proof.
-  iIntros "Hw Ht". iRevert (σ) "Hw". iRevert (t) "Ht".
-  iApply twptp_ind; iIntros "!#" (t) "IH"; iIntros (σ) "Hσ".
+  iIntros "Hσ Ht". iRevert (σ n) "Hσ". iRevert (t) "Ht".
+  iApply twptp_ind; iIntros "!#" (t) "IH"; iIntros (σ n) "Hσ".
   iApply (pure_mono _ _ (Acc_intro _)). iIntros ([t' σ'] [κ Hstep]).
-  iMod ("IH" with "[% //] Hσ") as (->) "[Hσ [H _]]".
+  rewrite /twptp_pre.
+  iMod ("IH" with "[% //] Hσ") as (n' ->) "[Hσ [H _]]".
   by iApply "H".
 Qed.
 End adequacy.
 
 Theorem twp_total Σ Λ `{invPreG Σ} s e σ Φ :
   (∀ `{Hinv : invG Σ},
-     (|={⊤}=> ∃ stateI : state Λ → list (observation Λ) -> iProp Σ,
-       let _ : irisG Λ Σ := IrisG _ _ _ Hinv stateI in
-       stateI σ [] ∗ WP e @ s; ⊤ [{ Φ }])%I) →
+     (|={⊤}=> ∃
+         (stateI : state Λ → list (observation Λ) → nat → iProp Σ)
+         (fork_post : iProp Σ),
+       let _ : irisG Λ Σ := IrisG _ _ _ Hinv stateI fork_post in
+       stateI σ [] 0 ∗ WP e @ s; ⊤ [{ Φ }])%I) →
   sn erased_step ([e], σ). (* i.e. ([e], σ) is strongly normalizing *)
 Proof.
   intros Hwp. apply (soundness (M:=iResUR Σ) _  2); simpl.
   apply (fupd_plain_soundness ⊤ _)=> Hinv.
-  iMod (Hwp) as (stateI) "[Hσ H]".
-  iApply (@twptp_total _ _ (IrisG _ _ _ Hinv stateI) with "Hσ").
-  by iApply (@twp_twptp _ _ (IrisG _ _ _ Hinv stateI)).
+  iMod (Hwp) as (stateI fork_post) "[Hσ H]".
+  iApply (@twptp_total _ _ (IrisG _ _ _ Hinv stateI fork_post) with "Hσ").
+  by iApply (@twp_twptp _ _ (IrisG _ _ _ Hinv stateI fork_post)).
 Qed.
