theories/program_logic/adequacy.v
@@ -39,14 +39,14 @@ Implicit Types P Q : iProp Σ.
 Implicit Types Φ : val Λ → iProp Σ.
 Implicit Types Φs : list (val Λ → iProp Σ).
 
-Notation wptp s t := ([∗ list] ef ∈ t, WP ef @ s; ⊤ {{ _, True }})%I.
+Notation wptp s t := ([∗ list] ef ∈ t, WP ef @ s; ⊤ {{ _, fork_post }})%I.
 
-Lemma wp_step s E e1 σ1 κ κs e2 σ2 efs Φ :
+Lemma wp_step s e1 σ1 κ κs e2 σ2 efs m Φ :
   prim_step e1 σ1 κ e2 σ2 efs →
-  state_interp σ1 (κ ++ κs) ∗ WP e1 @ s; E {{ Φ }}
-  ={E,∅}▷=∗ (state_interp σ2 κs ∗ WP e2 @ s; E {{ Φ }} ∗ wptp s efs).
+  state_interp σ1 (κ ++ κs) m -∗ WP e1 @ s; ⊤ {{ Φ }} ={⊤,∅}▷=∗
+  state_interp σ2 κs (length efs + m) ∗ WP e2 @ s; ⊤ {{ Φ }} ∗ wptp s efs.
 Proof.
-  rewrite {1}wp_unfold /wp_pre. iIntros (?) "[Hσ H]".
+  rewrite {1}wp_unfold /wp_pre. iIntros (?) "Hσ H".
   rewrite (val_stuck e1 σ1 κ e2 σ2 efs) //.
   iMod ("H" $! σ1 with "Hσ") as "(_ & H)".
   iMod ("H" $! e2 σ2 efs with "[//]") as "H".
@@ -55,43 +55,52 @@ Qed.
 
 Lemma wptp_step s e1 t1 t2 κ κs σ1 σ2 Φ :
   step (e1 :: t1,σ1) κ (t2, σ2) →
-  state_interp σ1 (κ ++ κs) ∗ WP e1 @ s; ⊤ {{ Φ }} ∗ wptp s t1
-  ==∗ ∃ e2 t2',
-    ⌜t2 = e2 :: t2'⌝ ∗ |={⊤,∅}▷=> (state_interp σ2 κs ∗ WP e2 @ s; ⊤ {{ Φ }} ∗ wptp s t2').
+  state_interp σ1 (κ ++ κs) (length t1) -∗ WP e1 @ s; ⊤ {{ Φ }} -∗ wptp s t1 ==∗
+  ∃ e2 t2', ⌜t2 = e2 :: t2'⌝ ∗
+  |={⊤,∅}▷=> state_interp σ2 κs (pred (length t2)) ∗ WP e2 @ s; ⊤ {{ Φ }} ∗ wptp s t2'.
 Proof.
-  iIntros (Hstep) "(HW & He & Ht)".
+  iIntros (Hstep) "Hσ He Ht".
   destruct Hstep as [e1' σ1' e2' σ2' efs [|? t1'] t2' ?? Hstep]; simplify_eq/=.
-  - iExists e2', (t2' ++ efs). iSplitR; first by eauto.
-    iFrame "Ht". iApply wp_step; eauto with iFrame.
+  - iExists e2', (t2' ++ efs). iModIntro. iSplitR; first by eauto.
+    iMod (wp_step with "Hσ He") as "H"; first done.
+    iIntros "!> !>". iMod "H" as "(Hσ & He2 & Hefs)".
+    iIntros "!>". rewrite Nat.add_comm app_length. iFrame.
   - iExists e, (t1' ++ e2' :: t2' ++ efs); iSplitR; first eauto.
-    iDestruct "Ht" as "($ & He' & $)". iFrame "He".
-    iApply wp_step; eauto with iFrame.
+    iFrame "He". iDestruct "Ht" as "(Ht1 & He1 & Ht2)".
+    iModIntro. iMod (wp_step with "Hσ He1") as "H"; first done.
+    iIntros "!> !>". iMod "H" as "(Hσ & He2 & Hefs)". iIntros "!>".
+    rewrite !app_length /= !app_length.
+    replace (length t1' + S (length t2' + length efs))
+      with (length efs + (length t1' + S (length t2'))) by omega. iFrame.
 Qed.
 
 Lemma wptp_steps s n e1 t1 κs κs' t2 σ1 σ2 Φ :
   nsteps n (e1 :: t1, σ1) κs (t2, σ2) →
-  state_interp σ1 (κs ++ κs') ∗ WP e1 @ s; ⊤ {{ Φ }} ∗ wptp s t1 ⊢
-  |={⊤,∅}▷=>^n (∃ e2 t2',
-    ⌜t2 = e2 :: t2'⌝ ∗ state_interp σ2 κs' ∗ WP e2 @ s; ⊤ {{ Φ }} ∗ wptp s t2').
+  state_interp σ1 (κs ++ κs') (length t1) -∗ WP e1 @ s; ⊤ {{ Φ }} -∗ wptp s t1
+  ={⊤,∅}▷=∗^n ∃ e2 t2',
+    ⌜t2 = e2 :: t2'⌝ ∗
+    state_interp σ2 κs' (pred (length t2)) ∗
+    WP e2 @ s; ⊤ {{ Φ }} ∗ wptp s t2'.
 Proof.
-  revert e1 t1 κs κs' t2 σ1 σ2; simpl; induction n as [|n IH]=> e1 t1 κs κs' t2 σ1 σ2 /=.
-  { inversion_clear 1; iIntros "(?&?&?)"; iExists e1, t1; iFrame; eauto 10. }
-  iIntros (Hsteps) "H". inversion_clear Hsteps as [|?? [t1' σ1']].
-  rewrite <- app_assoc.
-  iMod (wptp_step with "H") as (e1' t1'') "[% H]"; first eauto; simplify_eq.
-  iMod "H". iModIntro; iNext. iMod "H". iModIntro.
-  by iApply IH.
+  revert e1 t1 κs κs' t2 σ1 σ2; simpl.
+  induction n as [|n IH]=> e1 t1 κs κs' t2 σ1 σ2 /=.
+  { inversion_clear 1; iIntros "???"; iExists e1, t1; iFrame; eauto 10. }
+  iIntros (Hsteps) "Hσ He Ht". inversion_clear Hsteps as [|?? [t1' σ1']].
+  rewrite -(assoc_L (++)).
+  iMod (wptp_step with "Hσ He Ht") as (e1' t1'' ?) ">H"; first eauto; simplify_eq.
+  iIntros "!> !>". iMod "H" as "(Hσ & He & Ht)". iModIntro.
+  by iApply (IH with "Hσ He Ht").
 Qed.
 
-Lemma wptp_result s n e1 t1 κs κs' v2 t2 σ1 σ2 φ :
+Lemma wptp_result φ κs' s n e1 t1 κs v2 t2 σ1 σ2  :
   nsteps n (e1 :: t1, σ1) κs (of_val v2 :: t2, σ2) →
-  state_interp σ1 (κs ++ κs') ∗
-  WP e1 @ s; ⊤ {{ v, ∀ σ, state_interp σ κs' ={⊤,∅}=∗ ⌜φ v σ⌝ }} ∗
-  wptp s t1 ⊢
-  |={⊤,∅}▷=>^(S n) ⌜φ v2 σ2⌝.
+  state_interp σ1 (κs ++ κs') (length t1) -∗
+  WP e1 @ s; ⊤ {{ v, ∀ σ, state_interp σ κs' (length t2) ={⊤,∅}=∗ ⌜φ v σ⌝ }} -∗
+  wptp s t1 ={⊤,∅}▷=∗^(S n) ⌜φ v2 σ2⌝.
 Proof.
-  intros. rewrite Nat_iter_S_r wptp_steps //.
-  apply step_fupdN_mono.
+  iIntros (?) "Hσ He Ht". rewrite Nat_iter_S_r.
+  iDestruct (wptp_steps with "Hσ He Ht") as "H"; first done.
+  iApply (step_fupdN_wand with "H").
   iDestruct 1 as (e2 t2' ?) "(Hσ & H & _)"; simplify_eq.
   iMod (wp_value_inv' with "H") as "H".
   iMod (fupd_plain_mask_empty _ ⌜φ v2 σ2⌝%I with "[H Hσ]") as %?.
@@ -99,109 +108,166 @@ Proof.
   by iApply step_fupd_intro.
 Qed.
 
-Lemma wp_safe E e σ κs Φ :
-  state_interp σ κs -∗ WP e @ E {{ Φ }} ={E, ∅}▷=∗ ⌜is_Some (to_val e) ∨ reducible e σ⌝.
+Lemma wptp_all_result φ κs' s n e1 t1 κs v2 vs2 σ1 σ2 :
+  nsteps n (e1 :: t1, σ1) κs (of_val <$> v2 :: vs2, σ2) →
+  state_interp σ1 (κs ++ κs') (length t1) -∗
+  WP e1 @ s; ⊤ {{ v,
+    let m' := length vs2 in
+    state_interp σ2 κs' m' -∗ [∗] replicate m' fork_post ={⊤,∅}=∗ ⌜φ v ⌝ }} -∗
+  wptp s t1
+  ={⊤,∅}▷=∗^(S n) ⌜φ v2 ⌝.
+Proof.
+  iIntros (Hstep) "Hσ He Ht". rewrite Nat_iter_S_r.
+  iDestruct (wptp_steps with "Hσ He Ht") as "H"; first done.
+  iApply (step_fupdN_wand with "H").
+  iDestruct 1 as (e2 t2' ?) "(Hσ & H & Hvs)"; simplify_eq/=.
+  rewrite fmap_length. iMod (wp_value_inv' with "H") as "H".
+  iAssert ([∗] replicate (length vs2) fork_post)%I with "[> Hvs]" as "Hm".
+  { clear Hstep. iInduction vs2 as [|v vs] "IH"; csimpl; first by iFrame.
+    iDestruct "Hvs" as "[Hv Hvs]".
+    iMod (wp_value_inv' with "Hv") as "$". by iApply "IH". }
+  iMod (fupd_plain_mask_empty _ ⌜φ v2⌝%I with "[H Hm Hσ]") as %?.
+  { iApply ("H" with "Hσ Hm"). }
+  by iApply step_fupd_intro.
+Qed.
+
+Lemma wp_safe κs m e σ Φ :
+  state_interp σ κs m -∗
+  WP e {{ Φ }} ={⊤,∅}▷=∗ ⌜is_Some (to_val e) ∨ reducible e σ⌝.
 Proof.
   rewrite wp_unfold /wp_pre. iIntros "Hσ H".
   destruct (to_val e) as [v|] eqn:?.
-  { iApply (step_fupd_mask_mono ∅ _ _ ∅); eauto. set_solver. }
+  { iApply step_fupd_intro. set_solver. eauto. }
   iMod (fupd_plain_mask_empty _ ⌜reducible e σ⌝%I with "[H Hσ]") as %?.
-  { by iMod ("H" $! σ [] κs with "Hσ") as "($&H)". }
+  { by iMod ("H" $! σ [] κs with "Hσ") as "[$ H]". }
   iApply step_fupd_intro; first by set_solver+. 
   iIntros "!> !%". by right.
 Qed.
 
-Lemma wptp_safe n e1 κs κs' e2 t1 t2 σ1 σ2 Φ :
+Lemma wptp_safe κs' n e1 κs e2 t1 t2 σ1 σ2 Φ :
   nsteps n (e1 :: t1, σ1) κs (t2, σ2) → e2 ∈ t2 →
-  state_interp σ1 (κs ++ κs') ∗ WP e1 {{ Φ }} ∗ wptp NotStuck t1
-  ⊢ |={⊤,∅}▷=>^(S n) ⌜is_Some (to_val e2) ∨ reducible e2 σ2⌝.
+  state_interp σ1 (κs ++ κs') (length t1) -∗ WP e1 {{ Φ }} -∗ wptp NotStuck t1
+  ={⊤,∅}▷=∗^(S n) ⌜is_Some (to_val e2) ∨ reducible e2 σ2⌝.
 Proof.
-  intros ? He2. rewrite Nat_iter_S_r wptp_steps //.
-  apply step_fupdN_mono.
-  iDestruct 1 as (e2' t2' ?) "(Hw & H & Htp)"; simplify_eq.
-  apply elem_of_cons in He2 as [<-|?].
-  - iMod (wp_safe with "Hw H") as "$"; auto.
-  - iMod (wp_safe with "Hw [Htp]") as "$"; auto. by iApply (big_sepL_elem_of with "Htp").
+  iIntros (? He2) "Hσ He Ht". rewrite Nat_iter_S_r.
+  iDestruct (wptp_steps  with "Hσ He Ht") as "H"; first done.
+  iApply (step_fupdN_wand with "H").
+  iDestruct 1 as (e2' t2' ?) "(Hσ & H & Ht)"; simplify_eq.
+  apply elem_of_cons in He2 as [<-|(t1''&t2''&->)%elem_of_list_split].
+  - iMod (wp_safe with "Hσ H") as "$"; auto.
+  - iDestruct "Ht" as "(_ & He2 & _)". by iMod (wp_safe with "Hσ He2").
 Qed.
 
-Lemma wptp_invariance s n e1 κs κs' e2 t1 t2 σ1 σ2 φ Φ :
+Lemma wptp_invariance φ s n e1 κs κs' e2 t1 t2 σ1 σ2 Φ :
   nsteps n (e1 :: t1, σ1) κs (t2, σ2) →
-  (state_interp σ2 κs' ={⊤,∅}=∗ ⌜φ⌝) ∗
-  state_interp σ1 (κs ++ κs') ∗ WP e1 @ s; ⊤ {{ Φ }} ∗ wptp s t1
-  ⊢ |={⊤,∅}▷=>^(S n) |={⊤,∅}=> ⌜φ⌝.
+  (state_interp σ2 κs' (pred (length t2)) ={⊤,∅}=∗ ⌜φ⌝) -∗
+  state_interp σ1 (κs ++ κs') (length t1) -∗
+  WP e1 @ s; ⊤ {{ Φ }} -∗ wptp s t1
+  ={⊤,∅}▷=∗^(S n) ⌜φ⌝.
 Proof.
-  intros ?. rewrite Nat_iter_S_r wptp_steps // step_fupdN_frame_l.
-  apply step_fupdN_mono.
-  iIntros "[Hback H]"; iDestruct "H" as (e2' t2' ->) "[Hσ _]".
-  iSpecialize ("Hback" with "Hσ"). by iApply step_fupd_intro.
+  iIntros (?) "Hφ Hσ He Ht". rewrite Nat_iter_S_r.
+  iDestruct (wptp_steps _ n with "Hσ He Ht") as "H"; first done.
+  iApply (step_fupdN_wand with "H"). iDestruct 1 as (e2' t2' ->) "[Hσ _]".
+  iSpecialize ("Hφ" with "Hσ").
+  iMod (fupd_plain_mask_empty _ ⌜φ⌝%I with "Hφ") as %?.
+  by iApply step_fupd_intro.
 Qed.
 End adequacy.
 
 Theorem wp_strong_adequacy Σ Λ `{invPreG Σ} s e σ φ :
   (∀ `{Hinv : invG Σ} κs,
-     (|={⊤}=> ∃ stateI : state Λ → list (observation Λ) → iProp Σ,
-       let _ : irisG Λ Σ := IrisG _ _ _ Hinv stateI in
-       stateI σ κs ∗ WP e @ s; ⊤ {{ v, ∀ σ, stateI σ [] ={⊤,∅}=∗ ⌜φ v σ⌝ }})%I) →
+     (|={⊤}=> ∃
+         (stateI : state Λ → list (observation Λ) → nat → iProp Σ)
+         (fork_post : iProp Σ),
+       let _ : irisG Λ Σ := IrisG _ _ _ Hinv stateI fork_post in
+       (* This could be strengthened so that φ also talks about the number 
+       of forked-off threads *)
+       stateI σ κs 0 ∗ WP e @ s; ⊤ {{ v, ∀ σ m, stateI σ [] m ={⊤,∅}=∗ ⌜φ v σ⌝ }})%I) →
   adequate s e σ φ.
 Proof.
   intros Hwp; split.
   - intros t2 σ2 v2 [n [κs ?]]%erased_steps_nsteps.
-    eapply (step_fupdN_soundness' _ (S (S n)))=> Hinv.
-    rewrite Nat_iter_S.
-    iMod Hwp as (Istate) "[HI Hwp]".
-    iApply (step_fupd_mask_mono ∅ _ _ ∅); auto. iModIntro. iNext; iModIntro.
-    iApply (@wptp_result _ _ (IrisG _ _ _ Hinv Istate) _ _ _ _ _ []); eauto with iFrame.
+    eapply (step_fupdN_soundness' _ (S (S n)))=> Hinv. rewrite Nat_iter_S.
+    iMod (Hwp _ (κs ++ [])) as (stateI fork_post) "[Hσ Hwp]".
+    iApply step_fupd_intro; first done. iModIntro.
+    iApply (@wptp_result _ _ (IrisG _ _ _ Hinv stateI fork_post) with "[Hσ] [Hwp]"); eauto.
+    iApply (wp_wand with "Hwp"). iIntros (v) "H"; iIntros (σ'). iApply "H".
   - destruct s; last done. intros t2 σ2 e2 _ [n [κs ?]]%erased_steps_nsteps ?.
-    eapply (step_fupdN_soundness' _ (S (S n)))=> Hinv.
-    rewrite Nat_iter_S.
-    iMod Hwp as (Istate) "[HI Hwp]".
-    iApply (step_fupd_mask_mono ∅ _ _ ∅); auto.
-    iApply (@wptp_safe _ _ (IrisG _ _ _ Hinv Istate) _ _ _ []); [by eauto..|].
-    rewrite app_nil_r. eauto with iFrame.
+    eapply (step_fupdN_soundness' _ (S (S n)))=> Hinv. rewrite Nat_iter_S.
+    iMod (Hwp _ (κs ++ [])) as (stateI fork_post) "[Hσ Hwp]".
+    iApply step_fupd_intro; first done. iModIntro.
+    iApply (@wptp_safe _ _ (IrisG _ _ _ Hinv stateI fork_post) with "[Hσ] Hwp"); eauto.
 Qed.
 
 Theorem wp_adequacy Σ Λ `{invPreG Σ} s e σ φ :
   (∀ `{Hinv : invG Σ} κs,
      (|={⊤}=> ∃ stateI : state Λ → list (observation Λ) → iProp Σ,
-       let _ : irisG Λ Σ := IrisG _ _ _ Hinv stateI in
+       let _ : irisG Λ Σ := IrisG _ _ _ Hinv (λ σ κs _, stateI σ κs) True%I in
        stateI σ κs ∗ WP e @ s; ⊤ {{ v, ⌜φ v⌝ }})%I) →
   adequate s e σ (λ v _, φ v).
 Proof.
   intros Hwp. apply (wp_strong_adequacy Σ _)=> Hinv κs.
-  iMod Hwp as (stateI) "[Hσ H]". iExists stateI. iIntros "{$Hσ} !>".
+  iMod Hwp as (stateI) "[Hσ H]". iExists (λ σ κs _, stateI σ κs), True%I.
+  iIntros "{$Hσ} !>".
   iApply (wp_wand with "H"). iIntros (v ? σ') "_".
-  iMod (fupd_intro_mask' ⊤ ∅) as "_"; auto.
+  iIntros "_". by iApply fupd_mask_weaken.
+Qed.
+
+Theorem wp_strong_all_adequacy Σ Λ `{invPreG Σ} s e σ1 v vs σ2 φ :
+  (∀ `{Hinv : invG Σ} κs,
+     (|={⊤}=> ∃
+         (stateI : state Λ → list (observation Λ) → nat → iProp Σ)
+         (fork_post : iProp Σ),
+       let _ : irisG Λ Σ := IrisG _ _ _ Hinv stateI fork_post in
+       stateI σ1 κs 0 ∗ WP e @ s; ⊤ {{ v,
+         let m := length vs in
+         stateI σ2 [] m -∗ [∗] replicate m fork_post ={⊤,∅}=∗ ⌜ φ v ⌝ }})%I) →
+  rtc erased_step ([e], σ1) (of_val <$> v :: vs, σ2) →
+  φ v.
+Proof.
+  intros Hwp [n [κs ?]]%erased_steps_nsteps.
+  eapply (step_fupdN_soundness' _ (S (S n)))=> Hinv. rewrite Nat_iter_S.
+  iMod Hwp as (stateI fork_post) "[Hσ Hwp]".
+  iApply step_fupd_intro; first done. iModIntro.
+  iApply (@wptp_all_result _ _ (IrisG _ _ _ Hinv stateI fork_post)
+    with "[Hσ] [Hwp]"); eauto. by rewrite right_id_L.
 Qed.
 
 Theorem wp_invariance Σ Λ `{invPreG Σ} s e σ1 t2 σ2 φ :
   (∀ `{Hinv : invG Σ} κs κs',
-     (|={⊤}=> ∃ stateI : state Λ → list (observation Λ) → iProp Σ,
-       let _ : irisG Λ Σ := IrisG _ _ _ Hinv stateI in
-       stateI σ1 (κs ++ κs') ∗ WP e @ s; ⊤ {{ _, True }} ∗ (stateI σ2 κs' ={⊤,∅}=∗ ⌜φ⌝))%I) →
+     (|={⊤}=> ∃
+         (stateI : state Λ → list (observation Λ) → nat → iProp Σ)
+         (fork_post : iProp Σ),
+       let _ : irisG Λ Σ := IrisG _ _ _ Hinv stateI fork_post in
+       stateI σ1 (κs ++ κs') 0 ∗ WP e @ s; ⊤ {{ _, True }} ∗
+       (stateI σ2 κs' (pred (length t2)) ={⊤,∅}=∗ ⌜φ⌝))%I) →
   rtc erased_step ([e], σ1) (t2, σ2) →
   φ.
 Proof.
   intros Hwp [n [κs ?]]%erased_steps_nsteps.
-  eapply (step_fupdN_soundness _ (S (S n)))=> Hinv.
-  rewrite Nat_iter_S.
-  iMod (Hwp Hinv κs []) as (Istate) "(HIstate & Hwp & Hclose)".
+  apply (step_fupdN_soundness' _ (S (S n)))=> Hinv. rewrite Nat_iter_S.
+  iMod (Hwp Hinv κs []) as (Istate fork_post) "(Hσ & Hwp & Hclose)".
   iApply step_fupd_intro; first done.
-  iApply (@wptp_invariance _ _ (IrisG _ _ _ Hinv Istate)); eauto with iFrame.
+  iApply (@wptp_invariance _ _ (IrisG _ _ _ Hinv Istate fork_post)
+    with "Hclose [Hσ] [Hwp]"); eauto.
 Qed.
 
 (* An equivalent version that does not require finding [fupd_intro_mask'], but
 can be confusing to use. *)
 Corollary wp_invariance' Σ Λ `{invPreG Σ} s e σ1 t2 σ2 φ :
   (∀ `{Hinv : invG Σ} κs κs',
-     (|={⊤}=> ∃ stateI : state Λ → list (observation Λ) → iProp Σ,
-       let _ : irisG Λ Σ := IrisG _ _ _ Hinv stateI in
-       stateI σ1 κs ∗ WP e @ s; ⊤ {{ _, True }} ∗ (stateI σ2 κs' -∗ ∃ E, |={⊤,E}=> ⌜φ⌝))%I) →
+     (|={⊤}=> ∃
+         (stateI : state Λ → list (observation Λ) → nat → iProp Σ)
+         (fork_post : iProp Σ),
+       let _ : irisG Λ Σ := IrisG _ _ _ Hinv stateI fork_post in
+       stateI σ1 κs 0 ∗ WP e @ s; ⊤ {{ _, True }} ∗
+       (stateI σ2 κs' (pred (length t2)) -∗ ∃ E, |={⊤,E}=> ⌜φ⌝))%I) →
   rtc erased_step ([e], σ1) (t2, σ2) →
   φ.
 Proof.
   intros Hwp. eapply wp_invariance; first done.
-  intros Hinv κs κs'. iMod (Hwp Hinv) as (stateI) "(? & ? & Hφ)".
-  iModIntro. iExists stateI. iFrame. iIntros "Hσ".
+  intros Hinv κs κs'. iMod (Hwp Hinv) as (stateI fork_post) "(? & ? & Hφ)".
+  iModIntro. iExists stateI, fork_post. iFrame. iIntros "Hσ".
   iDestruct ("Hφ" with "Hσ") as (E) ">Hφ".
-  iMod (fupd_intro_mask') as "_"; last by iModIntro. solve_ndisj.
+  by iApply fupd_mask_weaken; first set_solver.
 Qed.
